%
% Chapter 11.5
%

\section*{11.5 Alternating Series}

\subsection*{Alternating Series Test}

If the alternating series
\[\sum_{n=1}^{\infty}{(-1)^{n-1}b_n} = b_1 - b_2 + b_3 - b_4 + b_5 - b_6
+ \cdots \quad b_n > 0\]
satisfies 
\begin{enumerate}
    \item \(b_{n+1} \leq b_n\) \quad for all \(n\)
    \item \(\lim_{n \to \infty}{b_n} = 0\)
\end{enumerate}
then the series if convergent.

\subsection*{Alternating Series Estimation Theorem}

If \(s = \sum{(-1)^{n-1}b_n}\), where \(b_n > 0\), is the sum of an alternating
series that satisfies
\[b_{n+1} \leq b_n \quad \text{ and } \quad \lim_{n \to \infty}{b_n} = 0\]
then
\[|R_n| = |s-s_n| \leq b_{n+1}\]
